Lean4Lean/Verify/Name.lean
@@ -1,0 +1,90 @@
+import Lean.Data.NameMap.Basic
+import Lean4Lean.Std.Ord
+import Std.Data.TreeSet.Lemmas
+
+/-!
+Order properties of `Lean.Name.cmp` and `Lean.Name.quickCmp`.
+-/
+
+namespace Lean
+
+namespace Name
+open _root_.Std Lean4Lean
+
+theorem cmp_eq_swap {a b : Name} : a.cmp b = (b.cmp a).swap := by
+  induction a generalizing b with obtain _|⟨b₁,b₂⟩|⟨b₁,b₂⟩ := b <;> simp [cmp]
+  | str a₁ a₂ ih | num a₁ a₂ ih =>
+    rw [ih]; cases b₁.cmp a₁ <;> simp [← OrientedOrd.eq_swap]
+
+instance : TransCmp cmp := by
+  refine TransCmp.of_rot (fun _ _ => cmp_eq_swap) fun a b c => ?_
+  induction a generalizing b c with
+  | anonymous =>
+    obtain _|⟨b₁,b₂⟩|⟨b₁,b₂⟩ := b <;> obtain _|⟨c₁,c₂⟩|⟨c₁,c₂⟩ := c <;> simp [cmp, Rot]
+  | str a₁ a₂ ih | num a₁ a₂ ih =>
+    obtain _|⟨b₁,b₂⟩|⟨b₁,b₂⟩ := b <;> obtain _|⟨c₁,c₂⟩|⟨c₁,c₂⟩ := c <;>
+      first
+      | exact (ih ..).then (Rot.of_transCmp ..)
+      | simp [cmp, Rot]
+
+instance : LawfulBEqCmp cmp where
+  compare_eq_iff_beq {a b} := by
+    simp; refine ⟨?_, fun h => h ▸ ReflCmp.compare_self⟩
+    induction a generalizing b with obtain _|⟨b₁,b₂⟩|⟨b₁,b₂⟩ := b <;> simp [cmp]
+    | str a₁ a₂ ih | num a₁ a₂ ih =>
+      refine ?_ ∘ Ordering.then_eq_eq.1
+      simp +contextual; exact fun h _ => ih h
+
+instance : TransCmp quickCmp where
+  eq_swap {a b} := by
+    simp [quickCmp]
+    rw [OrientedOrd.eq_swap]
+    cases compare b.hash a.hash <;> simp
+    induction a generalizing b with obtain _|⟨b₁,b₂⟩|⟨b₁,b₂⟩ := b <;> simp [quickCmpAux]
+    | str a₁ a₂ ih | num a₁ a₂ ih =>
+      rw [OrientedOrd.eq_swap]
+      cases compare b₂ a₂ <;> simp [ih]
+  isLE_trans {a b c} := by
+    have {α} [Ord α] [TransOrd α] {a₁ b₁ c₁ : α} {a₂ b₂ c₂}
+        (H : (quickCmpAux a₂ b₂).isLE → (quickCmpAux b₂ c₂).isLE → (quickCmpAux a₂ c₂).isLE) :
+        ((compare a₁ b₁).then (quickCmpAux a₂ b₂)).isLE →
+        ((compare b₁ c₁).then (quickCmpAux b₂ c₂)).isLE →
+        ((compare a₁ c₁).then (quickCmpAux a₂ c₂)).isLE := by
+      simp [Ordering.isLE_then_iff_and]
+      intro h1 h2 h3 h4
+      refine ⟨TransCmp.isLE_trans h1 h3, ?_⟩
+      refine h2.elim (fun h2 => .inl <| TransCmp.lt_of_lt_of_isLE h2 h3) fun h2 => ?_
+      refine h4.elim (fun h4 => .inl <| TransCmp.lt_of_isLE_of_lt h1 h4) fun h4 => .inr (H h2 h4)
+    apply this
+    induction a generalizing b c with
+      obtain _|⟨b₁,b₂⟩|⟨b₁,b₂⟩ := b <;> simp [quickCmpAux] at * <;>
+      obtain _|⟨c₁,c₂⟩|⟨c₁,c₂⟩ := c <;> simp [quickCmpAux] at *
+    | str a₁ a₂ ih | num a₁ a₂ ih => apply this ih
+
+instance : LawfulBEqCmp quickCmp where
+  compare_eq_iff_beq {a b} := by
+    simp; refine ⟨fun h => ?_, fun h => h ▸ ReflCmp.compare_self⟩
+    replace h := (Ordering.then_eq_eq.1 h).2; revert h
+    induction a generalizing b with obtain _|⟨b₁,b₂⟩|⟨b₁,b₂⟩ := b <;> simp [quickCmpAux]
+    | str a₁ a₂ ih | num a₁ a₂ ih =>
+      refine ?_ ∘ Ordering.then_eq_eq.1
+      simp +contextual; exact fun _ => ih
+
+end Name
+
+namespace NameSet
+open _root_.Std
+
+theorem contains_insert {s : NameSet} {a b : Name} :
+    (s.insert a).contains b = (a == b || s.contains b) := by
+  have key : (Name.quickCmp a b == Ordering.eq) = (a == b) := by
+    have := @LawfulBEqCmp.compare_eq_iff_beq _ _ Name.quickCmp _ a b
+    cases h : Name.quickCmp a b <;> simp_all
+  have h : (s.insert a).contains b
+      = (Name.quickCmp a b == Ordering.eq || s.contains b) :=
+    Std.TreeSet.contains_insert (t := s) (k := a) (a := b)
+  rw [h, key]
+
+@[simp] theorem contains_empty {a : Name} : (∅ : NameSet).contains a = false := rfl
+
+end NameSet
